% !TEX root=../../appendix.tex


% \begin{proof}[Proof of Theorem~\ref{thm:sound}]
%     \fixme{we cannot prove this, definition of drive function is incorrect}
% \end{proof}

\section{Soundness proofs}
\label{sec:soundness-proofs}

\subsection{Proof of soundness of symbolic evaluation semantics}
\begin{proof}
  We prove Lemma 6.5 by induction over the derivation of the symbolic evaluation $e,\sigma\simeval\overline{\sime,\sims,\phi}$.

  \case{\refrule{SE-Value}}
    {Since this case does not generate constraints, any $M$ will do.
    Since neither the state, nor the expression is altered by the evaluation rule \refrule{E-Value},
    this case holds trivially.
    }

\case{\refrule{SE-Fail}}
      {Since this case does not generate constraints, any $M$ will do.
      Since neither the state, nor the expression $\Fail$ is altered by the evaluation rule \refrule{E-Fail},
      this case holds trivially.
      }
  \case{\refrule{SE-Pair}}
    {For all mappings $M$ such that $M(\phi_1\wedge\phi_2)$,we need to demonstrate that
    $\tuple{e_1,e_2},\sigma\eval\tuple{v_1,v_2},\sigma''$ with
    $M\tuple{\simv_1,\simv_2} \equiv \tuple{v_1,v_2}$ and $M\sims''\equiv\sigma''$.

    From the induction hypothesis, we obtain the following.\\
    $\forall M_1 . \sime_1,\sims\simeval\overline{\simv_1,\sims',\phi_1}\land M_1\phi_1 \implies e_1,\sigma \eval v_1,\sigma'\land  M_1\simv_1\equiv v_1 \land  M_1\sims'\equiv\sigma'$ and
    $\forall M_2 . M_2\phi_2 \implies e_2, \sigma'\eval v_2,\sigma''\land M_2 \simv_2\equiv v_2\land M_2\sims''\equiv\sigma''$.

    Note that we have omitted from the second application of the induction hypothesis, the requirement that the symbolic step exists.
    The fact that this step exists is obtained from \refrule{SE-pair} and omitted to increase readability of this and any following proofs.

    Since $M$ satisfies both $\phi_1$ and $\phi_2$,
    we obtain from \refrule{E-Pair} and the induction steps above that $\tuple{e_1,e_2},\sigma\eval\tuple{v_1,v_2},\sigma''$, $M\tuple{\simv_1,\simv_2} \equiv \tuple{{v_1},{v_2}}$ and $M\sims''\equiv\sigma''$.
    }

\case{\refrule{SE-First}}
{
  For all mappings $M$ such that $M\phi$, we need to show that
  $\Fst e,\sigma\eval v_1,\sigma'$ with
  $M \simv_1\equiv {v_1}$ and $M\sims'\equiv{\sigma'}$.

  From the induction hypothesis, we obtain the following.\\
  $\forall M_1 . M_1\phi \implies e,\sigma\eval\tuple{v_1,v_2},\sigma'\land M_1\tuple{\simv_1,\simv_2}\equiv \tuple{{v_1},{v_2}}\land M_1\sims'\equiv{\sigma'}$

  Since $M$ satisfies $\phi$,
  we obtain from \refrule{E-First} and the induction step above that $\Fst e,\sigma\eval v_1,\sigma'$ with $M \simv_1\equiv v_1s$ and $M\sims'\equiv\sigma'$.
  }

\case{\refrule{SE-Second}}
{
  For all mappings $M$ such that $M\phi$, we need to show that
  $\Snd e,\sigma\eval v_2,\sigma'$ with $M \simv_2\equiv {v_2}$ and $M\sims'\equiv{\sigma'}$.

  From the induction hypothesis, we obtain the following.\\
  $\forall M_1 . M_1\phi \implies e, \sigma \eval\tuple{{v_1},{v_2}},{\sigma'}\land M_1\tuple{\simv_1,\simv_2}\equiv \tuple{{v_1},{v_2}}\land M_1\sims'\equiv{\sigma'}$

  Since $M$ satisfies $\phi$,
  we obtain from \refrule{E-Second} and the induction step above that $\Snd e,\sigma\eval v_2,\sigma'$ with
  $M \simv_2\equiv {v_2}$ and $M\sims'\equiv{\sigma'}$.
  }

\case{\refrule{SE-Cons}}
  {
  For all mappings $M$ such that $M\phi$, we need to demonstrate that
  $e_1 :: e_2,\sigma\eval v_1 :: v_2,\sigma''$ with
  $M \simv_1::\simv_2\equiv v_1 :: v_2$ and $M\sims''\equiv \sigma''$.

  From the induction hypothesis, we obtain the following.\\
  $\forall M_1 .  M_1\phi_1 \implies e_1, \sigma \eval v_1, \sigma' \land  M_1\simv_1\equiv{v_1} \land  M_1\sims'\equiv{\sigma'}$ and
  $\forall M_2 . M_2\phi_2 \implies e_2,\sigma' \eval v_2,\sigma'' \land M_2\simv_2\equiv{v_2} \wedge M_2\sims''\equiv{\sigma''}$

  Since $M$ satisfies both $\phi_1$ and $\phi_2$,
  we obtain from \refrule{E-Cons} and the induction steps above that $e_1 :: e_2,\sigma\eval v_1 :: v_2,\sigma''$ with $M(\simv_1::\simv_2) \equiv {v_1}::{v_2}$ and $M \sims'' \equiv{\sigma''}$.
  }

\case{\refrule{SE-Head}}
  {For all mappings $M$ such that $M\phi$, we need to show that
  $\Head e,\sigma\eval v_1,\sigma'$ with
  $M \simv_1\equiv {v_1}$ and $M\sims'\equiv{\sigma'}$.

  From the induction hypothesis, we obtain the following.\\
  $\forall M_1 . M_1\phi \implies e, \sigma\eval v_1 :: v_2 , \sigma' \land M_1 (\simv_1::\simv_2)\equiv {v_1}::{v_2}\land M_1\sims'\equiv{\sigma'}$

  Since $M$ satisfies $\phi$,
  we obtain from \refrule{E-Head} and the induction step above that $\Head e,\sigma{\eval}{v_1},\sigma'$ with
  $M \simv_1\equiv {v_1}$ and $M\sims'\equiv\sigma'$.}

\case{\refrule{SE-Tail}}
  { For all mappings $M$ such that $M\phi$, we need to show that
    $\Tail e,\sigma\eval v_2,\sigma'$ with
    $M \simv_2\equiv{v_2}$ and $M\sims'\equiv{\sigma'}$.

    From the induction hypothesis, we obtain the following.\\
    $\forall M_1 . M_1\phi \implies e, \sigma\eval {v_1}::{v_2},{\sigma'}\land M_1(\simv_1::\simv_2)\equiv {v_1}::{v_2}\land M_1\sims'\equiv{\sigma'}$

    Since $M$ satisfies $\phi$,
    we obtain from \refrule{E-Tail} and the induction step above that $\Tail e,\sigma{\eval}{v_2},\sigma'$ with
    $M \simv_2\equiv {v_2}$ and $M\sims'\equiv{\sigma'}$.}

\case{\refrule{SE-App}}
  {For all mappings $M$ such that $M(\phi_1 \land \phi_2\land \phi_3)$, we need to demonstrate that
  $e_1e_2,\sigma\eval v_1,\sigma'''$ with
   $M \simv_1 \equiv {v_1}$ and $M\sims'''\equiv{\sigma'''}$.

  From the induction hypothesis, we obtain the following.\\
  $\forall M_1 . M_1\phi_1 \implies e_1,\sigma{\eval}\lambda x : \tau.{e_1'},{\sigma'}
  \land M_1\lambda x : \tau.\sime_1' \equiv \lambda x : \tau.{e_1'} \land M_1\sims'\equiv{\sigma'}$
  and
  $\forall M_2 . M_2\phi_2 \implies e_2,\sigma'{\eval}{v_2},{\sigma''}
  \land M_2 \simv_2 \equiv {v_2} \land M_2\sims'' \equiv{\sigma''}$\\
  and
  $\forall M_3 . M_3\phi_3 \implies e_1'[x\mapsto {v_2}],\sigma''{\eval}{v_1},{\sigma'''}
  \land M_3 \simv_1\equiv {v_1} \land M_3 \sims'''\equiv{\sigma'''}$.

  Since $M$ satisfies $\phi_1$, $\phi_2$ and $\phi_3$, we obtain from \refrule{E-App} and the induction steps above that $e_1e_2,\sigma\eval v_1,\sigma'''$ with $M \simv_1 \equiv {v_1}$ and $M\sims'''\equiv{\sigma'''}$.
  }

\case{\refrule{SE-If}}
   {For all mappings $M$
   such that $M(\phi_1\land \phi_2 \land \simv_1)$, we need to demonstrate that
   $\If{e_1}{e_2}{e_3},\sigma\eval v_2,\sigma''$ with
   $M \simv_2 = {v_2}$ and $M\sims''=\sigma''$.

   From the induction hypothesis, we obtain the following.\\
   $\forall M_1 . M_1\phi_1 \implies e_1,\sigma\eval v_1,\sigma'
   \land M_1\simv_1 \equiv {v_1} \land M_1\sims'\equiv{\sigma'}$
   and
   $\forall M_2 . M_2\phi_2 \implies e_2,\sigma'\eval v_2,\sigma''
   \land M_2 \simv_2 \equiv {v_2} \land M_2\sims'' \equiv{\sigma''}$.

   Since $M$ satisfies $\phi_1$, $\phi_2$ and $\simv_1$, we know that $v_1=\True$.\\
   From \refrule{E-IfTrue} and the induction steps above, we obtain that
   $\If{e_1}{e_2}{e_3},\sigma\eval v_2,\sigma''$ with $M\simv_2={v_2}$ and $M\sims''={\sigma''}$.

   For all mappings $M$ such that $M(\phi_1\land \phi_3 \land \neg \simv_1)$,
   we need to demonstrate that
   $\If{e_1}{e_2}{e_3},\sigma\eval v_3,\sigma''$ with
   $M \simv_3 = {v_3}$ and $M\sims''={\sigma''}$.

   From the induction hypothesis, we obtain the following.\\
   $\forall M_1 . M_1\phi_1 \implies e_1,\sigma\eval{v_1},{\sigma'}
   \land M_1\simv_1 \equiv {v_1} \land M_1\sims'\equiv{\sigma'}$
   and
   $\forall M_3 . M_3\phi_3 \implies e_3,\sigma'\eval{v_3},{\sigma''}
   \land M_3 \simv_3 \equiv {v_3} \land M_3\sims'' \equiv{\sigma''}$.

   Since $M$ satisfies $\phi_1$, $\phi_3$ and $\neg\simv_1$, we know that $v_1=\False$.\\
   From \refrule{E-IfFalse} and the induction steps above, we obtain that
    $\If{e_1}{e_2}{e_3},\sigma\eval v_3,\sigma''$
   with $M\simv_3={v_3}$ and $M\sims''={\sigma''}$.
  }

\case{\refrule{SE-Ref}}
  {For all mappings $M$ such that $M\phi$,
  we need to demonstrate that
  $\Ref e,\sigma\eval l,\sigma'[l\mapsto v]$ with
  $M l \equiv l$ and $M\sims'[l\mapsto \simv]\equiv{\sigma'}[l\mapsto{v}]$.

  From the induction hypothesis, we obtain the following.\\
  $\forall M_1 .  M_1\phi \implies e, \sigma {\eval}{v},{\sigma'}\land  M_1\simv\equiv {v} \wedge  M_1\sims'\equiv{\sigma'}$.

  Since $M$ satisfies $\phi$,
  we obtain from \refrule{E-Ref} and the induction steps above that $\Ref e,\sigma\eval l,\sigma'[l\mapsto v]$.

  We assume that the assignment of location references happens in a deterministic manner, and that we can therefore conclude that exactly the same $l$ is used in both cases. Since $l$ cannot contain any symbols, $M l \equiv l$ holds trivially.

  This, together with $M \sims' \equiv{\sigma'}$ obtained from the induction hypothesis, we can conclude that $M\sims'[l\mapsto \simv]\equiv{\sigma'}[l\mapsto{v}]$.
  }

\case{\refrule{SE-Deref}}
  {For all mappings $M$ such that $M\phi$, we need to demonstrate that $!e,\sigma\eval\sigma'(l),\sigma'$ with
  $M \sims'(l) \equiv {\sigma'}(l)$ and $M\sims'\equiv{\sigma'}$.

  From the induction hypothesis, we obtain the following.\\
  $\forall M_1 .  M_1\phi \implies e, \sigma {\eval}l,{\sigma'}\land  M_1l\equiv l \land  M_1\sims'\equiv{\sigma'}$.

  Since $M$ satisfies $\phi$,
  we obtain from \refrule{E-Deref} and the induction step above that $!e,\sigma {\eval}\sigma'(l),{\sigma'}$ with $M \sims'(l) \equiv {\sigma'}(l)$
  and $M\sims'\equiv{\sigma'}$.
}

\case{\refrule{SE-Assign}}
  {
  For all mappings $M$ such that $M(\phi_1\wedge \phi_2)$,
  we need to demonstrate that\\
  $e_1 := e_2,\sigma\eval\unit,\sigma''[l\mapsto v_2]$ with
  $M\unit \equiv \unit$, which holds true trivially,
  and $M\sims''[l\mapsto \simv_2]\equiv{\sigma''}[l\mapsto{v_2}]$.

  From the induction hypothesis, we obtain the following.\\
  $\forall M_1 .  M_1\phi_1 \implies e_1, \sigma {\eval}l,{\sigma'}\land  M_1 l\equiv l \land  M_1\sims'\equiv{\sigma'}$ and
  $\forall M_2 . M_2\phi_2 \implies e_2,\sigma' {\eval}{v_2},{\sigma''}\land M_2\simv_2\equiv {v_2} \land M_2\sims''\equiv{\sigma''}$

  Since $M$ satisfies both $\phi_1$ and $\phi_2$, we obtain from \refrule{E-Assign} and the induction steps above that $e_1 := e_2,\sigma\eval\unit,\sigma''[l\mapsto v_2]$ with $M\sims''[l\mapsto \simv_2]\equiv{\sigma''}[l\mapsto{v_2}]$.
  }

\case{\refrule{SE-Edit}}
  {For all mappings $M$ such that $M\phi$,
  we need to demonstrate that $\Edit e,\sigma\eval\Edit v,\sigma'$ with
  $M \Edit \simv \equiv \Edit {v}$ and $M\sims'\equiv{\sigma'}$.

  From the induction hypothesis, we obtain the following.
  $\forall M_1 .  M_1\phi \implies e, \sigma {\eval}{v},{\sigma'}\land  M_1\simv\equiv {v} \land  M_1\sims'\equiv{\sigma'}$.

  Since $M$ satisfies $\phi$,
  we obtain from \refrule{E-Edit} and the induction step above that $\Edit e,\sigma\eval\Edit v,\sigma'$ with $M \Edit \simv\equiv \Edit {v}$ and $ M\sims'\equiv{\sigma'}$.

  }

\case{\refrule{SE-Update}}
  {For all mappings $M$ such that $M\phi$, we need to demonstrate that $\Update e,\sigma\eval\Update l,\sigma'$ with
  $M \Update l \equiv \Update l$ and $M\sims'\equiv{\sigma'}$.

  From the induction hypothesis, we obtain the following.
  $\forall M_1 .  M_1\phi \implies e, \sigma {\eval}l,{\sigma'}\land  M_1 l\equiv l \land  M_1\sims'\equiv{\sigma'}$.

  Since $M$ satisfies $\phi$,
  we obtain from \refrule{E-Update} and the induction step above that $\Update e,\sigma\eval\Update l,\sigma'$ with $M \Update l\equiv \Update l$ and $M \sims' \equiv{\sigma'}$.

  }

\case{\refrule{SE-Then}}
  {For all mappings $M$ such that $M\phi$, we need to demonstrate that
  $e_1\Then e_2,\sigma\eval t_1\Then e_2,\sigma'$ with
  $M \simt_1\Then \sime_2 \equiv {t_1}\Then e_2$ and $M\sims'\equiv{\sigma'}$.

  From the induction hypothesis, we obtain the following.
  $\forall M_1 .  M_1\phi \implies e, \sigma {\eval}{t_1},{\sigma'}\land  M_1 \simt_1\equiv {t_1} \land  M_1\sims'\equiv{\sigma'}$.

  Since $M$ satisfies $\phi$,
  we obtain from \refrule{E-Then} and the induction step above that $e_1\Then e_2,\sigma\eval t_1\Then e_2,\sigma'$ with $M \simt_1\Then \sime_2 \equiv {t_1}\Then e_2$ and $M \sims' \equiv\sigma'$.

  }

\case{\refrule{SE-Next}}
  {For all mappings $M$ such that $M\phi$, we need to demonstrate that
  $e_1\Next e_2,\sigma\eval t_1\Next e_2,\sigma'$ with
  $M \simt_1\Next e_2 \equiv {t_1}\Next e_2$ and $M\sims'\equiv{\sigma'}$.

  From the induction hypothesis, we obtain the following.
  $\forall M_1 .  M_1\phi \implies e,\sigma {\eval}{t_1},{\sigma'}\land  M_1 \simt_1\equiv {t_1} \land  M_1\sims'\equiv{\sigma'}$.

  Since $M$ satisfies $\phi$,
  we obtain from \refrule{E-Next} and the induction step above that $e_1\Next e_2,\sigma\eval t_1\Next e_2,\sigma'$ with $M \simt_1\Next e_2 \equiv {t_1}\Next e_2$ and $M \sims' \equiv{\sigma'}$.

  }

\case{\refrule{SE-Or}}
  {For all mappings $M$ such that $M(\phi_1\wedge \phi_2)$, we need to demonstrate that
   $e_1\Or e_2,\sigma\eval t_1\Or t_2,\sigma''$ with $M \simt_1\Or \simt_2 \equiv {t_1}\Or{t_2}$ and $M\sims''\equiv{\sigma''}$.

  From the induction hypothesis, we obtain the following.\\
  $\forall M_1 .  M_1\phi_1 \implies e_1, \sigma {\eval}{t_1},{\sigma'}\land  M_1 \simt_1\equiv {t_1} \land  M_1\sims'\equiv{\sigma'}$ and
  $\forall M_2 . M_2\phi_2 \implies e_2,\sigma' {\eval}{t_2},{\sigma''}\land M_2\simt_2\equiv {t_2} \land M_2\sims''\equiv{\sigma''}$

  Since $M$ satisfies both $\phi_1$ and $\phi_2$, we obtain from \refrule{E-Or} and the induction steps above that $e_1\Or e_2,\sigma\eval t_1\Or t_2,\sigma''$ with $M \simt_1\Or \simt_2 \equiv {t_1}\Or{t_2}$ and $M \sims'' \equiv{\sigma''}$.

  }

  \case{\refrule{SE-And}}
    {For all mappings $M$ such that $M(\phi_1\wedge \phi_2)$, we need to demonstrate that
     $e_1\And e_2,\sigma\eval t_1\And t_2,\sigma''$ with $M \simt_1\And \simt_2 \equiv {t_1}\And{t_2}$ and $M\sims''\equiv{\sigma''}$.

    From the induction hypothesis, we obtain the following.\\
    $\forall M_1 .  M_1\phi_1 \implies e_1, \sigma {\eval}{t_1},{\sigma'}\land  M_1 \simt_1\equiv {t_1} \land  M_1\sims'\equiv{\sigma'}$ and
    $\forall M_2 . M_2\phi_2 \implies e_2,\sigma' {\eval}{t_2},{\sigma''}\land M_2\simt_2\equiv {t_2} \land M_2\sims''\equiv{\sigma''}$

    Since $M$ satisfies both $\phi_1$ and $\phi_2$, we obtain from \refrule{E-And} and the induction steps above that $e_1\And e_2,\sigma\eval t_1\And t_2,\sigma''$ with $M \simt_1\And \simt_2 \equiv {t_1}\And{t_2}$ and $M \sims'' \equiv{\sigma''}$.

    }

\end{proof}


\subsection{Proof of soundness of symbolic striding semantics}
\begin{proof}
  We prove Lemma 6.4 by induction over the derivation $t,\sigma\simstride\overline{\simt,\sims,\phi}$.

  \case{\refrule{SS-ThenStay},\refrule{SS-ThenFail}}
    {For all mappings $M$ such that $M\phi$
    we need to demonstrate that
    $t_1\Then e_2,\sigma\stride  t_1'\Then e_2,\sigma'$ with
    $M \simt_1'\Then e_2 \equiv {t_1'}\Then e_2 $ and $ M\sims'\equiv {\sigma'}$.

    From the induction hypothesis, we obtain the following.
    $\forall M_1 . M_1 \phi \implies t_1,\sigma {\stride} {t_1'},{\sigma'}\land M_1 \simt_1'\equiv{t_1'}\land M_1\sims' \equiv {\sigma'}$.

    Since $M$ satisfies $\phi$,
    we obtain from \refrule{S-ThenStay} and \refrule{S-ThenFail} respectively, and the induction step above that $t_1\Then e_2,\sigma\stride  t_1'\Then e_2,\sigma'$ with
    $M \simt_1'\Then e_2 \equiv {t_1'}\Then e_2 $ and $ M\sims'\equiv {\sigma'}$.
    }

  \case{\refrule{SS-ThenCont}}
    {For all mappings $M$ such that $M\phi_1\land M\phi_2$
    we need to demonstrate that
    $t_1\Then e_2,\sigma\stride t_2,\sigma''$ with
    $M \simt_2 \equiv {t_2}$ and $M\sims''\equiv {\sigma''}$.

    From the induction hypothesis, we obtain the following.
    $\forall M_1 . M_1 \phi_1 \implies t_1,\sigma {\stride} {t_1'},{\sigma'}\implies M_1 \simt_1'\equiv{t_1'}\land M_1\sims' \equiv {\sigma'}$.\\
    From Lemma 6.5 we know that
    $\forall M_2 . M_2 \phi_2 \implies e_2{v_1},\sigma'{\eval}{t_2},{\sigma''}\and M_2 \simt_2\equiv {t_2}\land M_2\sims''\equiv {\sigma''}$.

    Since $M$ satisfies both $\phi_1$ and $\phi_2$,
    we obtain from \refrule{S-ThenCont}, the induction step and application of Lemma 6.5 above that
    $t_1\Then e_2,\sigma\stride t_2,\sigma''$ with
    $M \simt_2 \equiv t_2$ and $M\sims''\equiv {\sigma''}$.
    }

  \case{\refrule{SS-OrLeft}}
    {For all mappings $M$ such that $M\phi$
    we have to demonstrate that
    $t_1\Or t_2,\sigma\stride t_1',\sigma'$ with
    $M \simt_1'\equiv {t_1'}$ and $M\sims'\equiv {\sigma'}$.

    From the induction hypothesis, we obtain the following.
    $\forall M_1 . M_1 \phi \implies t_1,\sigma {\stride} {t_1'},{\sigma'}\and M_1 \simt_1'\equiv{t_1'}\land M_1\sims' \equiv {\sigma'}$.

    Since $M$ satisfies $\phi$, we obtain from \refrule{S-OrLeft} and the induction step above that $t_1\Or t_2,\sigma\stride t_1',\sigma'$ with
    $M \simt_1'\equiv{t_1'}$ and $M\sims'\equiv {\sigma'}$.

    }

  \case{\refrule{SS-OrRight}}
    {For all mappings $M$ such that $M(\phi_1\land \phi_2)$
    we need to demonstrate that
    $t_1\Or t_2,\sigma\stride t_2',\sigma''$ with
    $M \simt_2'\equiv {t_2'}$ and $M\sims''\equiv {\sigma''}$.

    From the induction hypothesis, we obtain the following.\\
    $\forall M_1 . M_1 \phi_1 \implies t_1,\sigma {\stride} {t_1'},{\sigma'}\land M_1 \simt_1'\equiv{t_1'}\land M_1\sims' \equiv {\sigma'}$ and
    $\forall M_2 . M_2 \phi_2 \implies t_2,\sigma' {\stride} {t_2'},{\sigma''}\land M_2 \simt_2'\equiv{t_2'}\land M_2\sims'' \equiv {\sigma''}$.

    Since $M$ satisfies both $\phi_1$ and $\phi_2$, and from the premise we have that $\Value\ (\simt',\sims')=\bot$,
    we obtain from \refrule{S-OrRight} and the induction steps above that $t_1\Or t_2,\sigma\stride t_2',\sigma''$ with
    $M \simt_2'\equiv{t_2'}$ and $M\sims''\equiv{\sigma''}$.
    }

  \case{\refrule{SS-OrNone}}
    {For all mappings $M$ such that $M(\phi_1\land \phi_2)$
    we need to demonstrate that $t_1\Or t_2,\sigma\stride t_1'\Or t_2',\sigma''$ with
    $M \simt_1'\Or \simt_2'\equiv {t_1'}\Or{t_2'}$ and $M\sims''\equiv {\sigma''}$.

    From the induction hypothesis, we obtain the following.\\
    $\forall M_1 . M_1 \phi_1 \implies t_1,\sigma {\stride} {t_1'},{\sigma'}\land M_1 \simt_1'\equiv{t_1'}\land M_1\sims' \equiv {\sigma'}$ and
    $\forall M_2 . M_2 \phi_2 \implies t_2,\sigma' {\stride} {t_2'},{\sigma''}\land M_2 \simt_2'\equiv{t_2'}\land M_2\sims'' \equiv {\sigma''}$.

    Since $M$ satisfies both $\phi_1$ and $\phi_2$,
    we obtain from \refrule{S-OrNone} and the induction steps above that $t_1\Or t_2,\sigma\stride t_1'\Or t_2',\sigma''$ with
    $M \simt_1'\Or \simt_2'\equiv {t_1'}\Or{t_2'}$ and $M\sims''\equiv {\sigma''}$.

    }

\case{\refrule{SS-Edit}}
  {For all mappings $M$, we need to demonstrate that
  $\Edit v,\sigma\stride \Edit v,\sigma$ with $M\Edit v \equiv \Edit v$ and $M\sigma \equiv \sigma$.
  This follows trivially from \refrule{S-Edit}.

  }

\case{\refrule{SS-Fill}}
  {For all mappings $M$, we need to demonstrate that $\Enter\beta,\sigma\stride\Enter\beta,\sigma$ with
  $M\Enter \beta \equiv \Enter \beta$ and $M\sigma \equiv {\sigma}$.
  This follows trivially from \refrule{S-Fill}.
  }

\case{\refrule{SS-Update}}
  {For all mappings $M$, we need to demonstrate that $\Update l,\sigma\stride\Update l,\sigma$ with
  $M\Update l \equiv \Update l$ and $M\sigma \equiv {\sigma}$.
  This follows trivially from \refrule{S-Update}.
  }

\case{\refrule{SS-Fail}}
  {For all mappings $M$, we need to demonstrate that $\Fail,\sigma\stride\Fail,\sigma$
  with
  $M\Fail \equiv \Fail$ and $M\sigma \equiv {\sigma}$.
  This follows trivially from \refrule{S-Fail}.
  }

\case{\refrule{SS-Xor}}
  {For all mappings $M$, we need to demonstrate that $e_1\Xor e_2,\sigma\stride e_1\Xor e_2,\sigma$ with
  $M e_1\Xor e_2 \equiv e_1\Xor e_2$ and $M\sims \equiv {\sigma}$.
  This follows trivially from \refrule{S-Xor}.
  }

\case{\refrule{SS-Next}}
  {For all mappings $M$ such that $M\phi$,
  we need to demonstrate that
  $t_1\Next e_2,\sigma\stride t_1'\Next e_2,\sigma'$ with
  $M \simt_1'\Next e_2\equiv {t_1'}\Next e_2$ and $M \sims'\equiv{\sigma'}$.

  From the induction hypothesis, we obtain the following.
  $\forall M_1 . M_1 \phi \implies t_1,\sigma {\stride} {t_1'},{\sigma'}\land M_1 \simt_1'\equiv{t_1'}\land M_1\sims' \equiv{\sigma'}$.

  Since $M$ satisfies $\phi$, we obtain from \refrule{S-Next} and the induction step above that $t_1\Next e_2,\sigma\stride t_1'\Next e_2,\sigma'$ with
  $M \simt_1'\Next e_2\equiv {t_1'}\Next e_2$ and $M \sims'\equiv{\sigma'}$.

  }

\case{\refrule{SS-And}}
  {For all mappings $M$ such that $M(\phi_1\land \phi_2)$
  we need to demonstrate that $t_1\And t_2,\sigma\stride t_1'\And t_2',\sigma''$ with
  $M \simt_1'\And \simt_2'\equiv {t_1'}\And{t_2'}$ and $M\sims''\equiv {\sigma''}$.

  From the induction hypothesis, we obtain the following.\\
  $\forall M_1 . M_1 \phi_1 \implies t_1,\sigma {\stride} {t_1'},{\sigma'}\and M_1 \simt_1'\equiv{t_1'}\land M_1\sims' \equiv {\sigma'}$ and
  $\forall M_2 . M_2 \phi_2 \implies t_2,\sigma' {\stride} {t_2'},{\sigma''}\and M_2 \simt_2'\equiv{t_2'}\land M_2\sims'' \equiv {\sigma''}$.

  Since $M$ satisfies both $\phi_1$ and $\phi_2$,
  we obtain from \refrule{S-And} and the induction steps above that $t_1\And t_2,\sigma\stride t_1'\And t_2',\sigma''$ with
  $M \simt_1'\And \simt_2'\equiv {t_1'}\And{t_2'}$ and $M\sims''\equiv {\sigma''}$.

  }

\end{proof}


\subsection{Proof of soundness of symbolic normalisation semantics}
\begin{proof}
  We prove Lemma 6.3 by induction over the derivation $e,\sigma\simnormalise \overline{\simt,\sims,\phi}$.

  The base case is when the SN-Done rule applies.
  Provided that $M(\phi_1\land \phi_2)$,
  we need to demonstrate that
  $e,\sigma\normalise t,\sigma'$ with
  $M \simt\equiv {t}$ and $M\sims'\equiv {\sigma'}$.

  By Lemma 6.5 and 6.4, we know that\\
  $\forall M_1. M_1\phi_1 \implies e,\sigma {\eval}{t},{\sigma'}\land M_1 \simt \equiv {t} \land M_1 \sims'\equiv {\sigma'}$ and
  $\forall M_2.M_2\phi_2\implies t,\sigma'{\stride}{t'},{\sigma''}\land M_2 \simt'\equiv{t'}\land M_2\sims''\equiv {\sigma''}$.

  Since $M$ satisfies both $\phi_1$ and $\phi_2$, we have $e,\sigma \normalise {t},{\sigma'}$ with $M\sims'\equiv {\sigma'}$.

  The induction step is when \refrule{SN-Repeat} applies.
  In this case, for all mappings $M$ such that
  $M(\phi_1\land \phi_2 \land \phi_3)$,
  we need to demonstrate that $e,\sigma\normalise t'',\sigma'''$
  with $M \simt''\equiv {t''}$ and $M\sims'''\equiv {\sigma'''}$.

  Again by Lemma 6.5 and 6.4, we know that\\
  $\forall M_1. M_1\phi_1 \implies e,\sigma {\eval}{t},{\sigma'}\land M_1 \simt \equiv {t} \land M_1 \sims'\equiv {\sigma'}$ and
  $\forall M_2.M_2\phi_2\implies t,\sigma'{\stride}{t'},{\sigma''}\land M_2 \simt'\equiv{t'}\land M_2\sims''\equiv {\sigma''}$.\\
  Furthermore, we know by applying the induction hypothesis that
  $\forall M_3.M_3\phi_3 \implies t',\sigma''{\normalise} {t''},{\sigma'''}\land M_3 \simt''\equiv {t''}\land M_3 \sims'''\equiv {\sigma'''}$.

  Since $M$ satisfies $\phi_1$, $\phi_2$ and $\phi_3$,
  we obtain from \refrule{N-Repeat}, the application of lemmas and the induction step above that $e,\sigma\normalise t'',\sigma'''$
  with $M \simt''\equiv {t''}$ and $M\sims'''\equiv {\sigma'''}$.
\end{proof}

\subsection{Proof of soundness of symbolic handling semantics}

\label{appendix:symbolicsoundhandle}
\begin{proof}
  We prove Lemma 6.2 by induction over the derivation $t,\sigma\simhandle\simt,\sims,\simi,\phi$.

  \case{\refrule{SH-Change}}
    {
    For all mappings $M$, we need to demonstrate that $\Edit v,\sigma\handle{M s}\Edit M s,\sigma$ with $M\Edit s\equiv \Edit M s$ and $ M\sigma\equiv {\sigma}$.

    This follows trivially from \refrule{H-Change}.

    }

  \case{\refrule{SH-Fill}}
  {For all mappings $M$, we need to demonstrate that
  $\Enter\beta,\sigma\handle{M s} \Edit M s,\sigma$ with
  $M \Edit s \equiv \Edit M s$ and $ M\sigma\equiv {\sigma}$.

  This follows trivially from \refrule{H-Fill}.

  }

  \case{\refrule{SH-Update}}
  {
  For all mappings $M$,
  we need to demonstrate that\\
  $\Update l,\sigma\handle{M s}\Update l,\sigma[l\mapsto M s]$ with
  $M \Update l \equiv \Update l$ and $ M\sigma[l\mapsto s]\equiv {\sigma}[l\mapsto M s]$.

  $\Update l,\sigma\handle{M s}\Update l,\sigma[l\mapsto M s]$ follows trivially from \refrule{H-Update}.
  $M \Update l \equiv \Update l$ follows trivially, since locations cannot contain symbols.
  $ M\sigma[l\mapsto s]\equiv {\sigma}[l\mapsto M s]$ follows trivially.

  }

  \case{\refrule{SH-Next}}

  {For all mappings $M$ such that $M\phi_1$, we need to demonstrate that
  $t_1\Next e_2,\sigma\handle{M \simi} t_1'\Next e_2,\sigma'$ with
  $M \simt_1' \Next e_2 \equiv {t_1'}\Next e_2$ and $M\sims'\equiv{\sigma'}$.

  By the induction hypothesis we obtain the following.
  $\forall M_1 . M_1 \phi_1 \implies t_1,\sigma \handle{M_1 \simi} {t_1'},{\sigma'}\land M_1 \simt_1'\equiv{t_1'}\land M_1\sims' \equiv {\sigma'}$

  Since $M$ satisfies $\phi_1$, we obtain from \refrule{H-PassNext} and the induction step above that $t_1\Next e_2,\sigma\handle{M \simi} t_1'\Next e_2,\sigma'$ with
  $M \simt_1' \Next e_2 \equiv {t_1'}\Next e_2$ and $M\sims'\equiv{\sigma'}$.



  For all mappings $M$ such that $M\phi_2$, we need to demonstrate that
  $t_1\Next e_2,\sigma\handle{\Continue}t_2,\sigma'$ with
  $M \simt_2 \equiv {t_2}$ and $M\sims'\equiv{\sigma'}$.

  From Lemma 6.3 we obtain that $\forall M_1. M_1 \phi \implies e_2 v_1,\sigma{\normalise}{t_2},{\sigma'}\land M \simt_2\equiv{t_2}\land M \sims'\equiv{\sigma'}$.

  This together with \refrule{H-Next} gives us exactly what we need to prove this case.
    }

  \case{\refrule{SH-PassNext}}
  {
  For all mappings $M$ such that $M\phi$, we need to demonstrate that
  $t_1\Next e_2,\sigma\handle{M\simi}t_1'\Next e_2,\sigma'$ with
  $M \simt_1' \Next e_2 \equiv {t_1'}\Next e_2$ and $M\sims'\equiv{\sigma'}$.

  By the induction hypothesis we obtain the following.
  $\forall M_1 . M_1 \phi_1 \implies t_1,\sigma \handle{M_1 \simi} {t_1'},{\sigma'}\land M_1 \simt_1'\equiv{t_1'}\land M_1\sims' \equiv {\sigma'}$

  Since $M$ satisfies $\phi$, we obtain from \refrule{H-PassNext} and the induction step above that $t_1\Next e_2,\sigma\handle{M\simi}t_1'\Next e_2,\sigma'$ with
  $M \simt_1' \Next e_2 \equiv {t_1'}\Next e_2$ and $M\sims'\equiv{\sigma'}$.
  }

    \case{\refrule{SH-PassNextFail}}
    {
    For all mappings $M$ such that $M\phi$, we need to demonstrate that
    $t_1\Next e_2,\sigma\handle{M\simi}t_1'\Next e_2,\sigma'$ with
    $M \simt_1' \Next e_2 \equiv {t_1'}\Next e_2$ and $M\sims'\equiv{\sigma'}$.

    By the induction hypothesis we obtain the following.
    $\forall M_1 . M_1 \phi_1 \implies t_1,\sigma \handle{M_1 \simi} {t_1'},{\sigma'}\land M_1 \simt_1'\equiv{t_1'}\land M_1\sims' \equiv {\sigma'}$.

    Since $M$ satisfies $\phi$ and from the premise of \refrule{SH-PassNextFail} we have $\Failing\ (\simt_2,\sims'')$, we obtain from \refrule{H-PassNextFail} and the induction step above that $t_1\Next e_2,\sigma\handle{M\simi}t_1'\Next e_2,\sigma'$ with
    $M \simt_1' \Next e_2 \equiv {t_1'}\Next e_2$ and $M\sims'\equiv{\sigma'}$.
    }

  \case{\refrule{SH-PassThen}}
  {For all mappings $M$ such that $M\phi$, we need to demonstrate that
  $t_1\Then e_2,\sigma\handle{M\simi}t_1'\Then e_2,\sigma'$ with
  $M \simt_1'\Then e_2\equiv {t_1'}\Then e_2$ and $M\sims'\equiv{\sigma'}$.

  By the induction hypothesis we obtain the following.
  $\forall M_1 . M_1 \phi_1 \implies t_1,\sigma \handle{M_1 \simi} {t_1'},{\sigma'}\land M_1 \simt_1'\equiv{t_1'}\land M_1\sims' \equiv {\sigma'}$

  Since $M$ satisfies $\phi$, we obtain from \refrule{H-PassThen} and the induction step above that $t_1\Then e_2,\sigma\handle{M\simi}t_1'\Then e_2,\sigma'$ with
  $M \simt_1'\Then e_2\equiv {t_1'}\Then e_2$ and $M\sims'\equiv{\sigma'}$.
  }

    \case{\refrule{SH-Pick}}
    {
    We have that $M\phi_1$ and/or $M\phi_2$.
    In the first case, the proof is identical to the SH-PickLeft rule.
    In the second case, the proof is identical to the SH-PickRight rule.
    }

    \case{\refrule{SH-PickLeft}}
    {For all mappings $M$ such that  $M\phi_1$, we need to demonstrate that
    $e_1\Xor e_2,\sigma\handle{\Left}t_1,\sigma'$ with
    $M \simt_1\equiv {t_1}$ and $M\sims'\equiv {\sigma'}$.

    From Lemma 6.3 we obtain that $\forall M_1. M_1 \phi \implies e_1,\sigma{\normalise}{t_1},{\sigma'}\land M \simt_1\equiv{t_1}\land M \sims'\equiv{\sigma'}$.

    Since $M$ satisfies $\phi_1$, we obtain from \refrule{H-PickLeft} and the application of Lemma 6.3 above that $e_1\Xor e_2,\sigma\handle{\Left}t_1,\sigma'$ with
    $M \simt_1\equiv {t_1}$ and $M\sims'\equiv {\sigma'}$.
    }

    \case{\refrule{SH-PickRight}}
    {For all mappings $M$ such that $M\phi_2$, we need to demonstrate that
    $e_1\Xor e_2,\sigma\handle{\Right}t_2,\sigma'$ with
    $M \simt_2\equiv {t_2}$ and $M\sims_2\equiv {\sigma'}$.

    From Lemma 6.3 we obtain that $\forall M_1. M_1 \phi \implies e_2,\sigma{\normalise}{t_2},{\sigma'}\land M \simt_2\equiv{t_2}\land M \sims'\equiv{\sigma'}$.

    Since $M$ satisfies $\phi_2$, we obtain from \refrule{H-PickRight} and the application of Lemma 6.3 above that $e_1\Xor e_2,\sigma\handle{\Right}t_2,\sigma'$ with
    $M \simt_2\equiv {t_2}$ and $M\sims_2\equiv {\sigma'}$.
    }

  \case{\refrule{SH-And}}
  {For all mappings $M$ such that $M\phi_1$, we need to demonstrate that
   $t_1\And t_2,\sigma\handle{M\First \simi}t_1'\And t_2,\sigma'$ with
   $M \simt_1'\And t_2\equiv {t_1'}\And t_2$ and $M\sims'\equiv {\sigma'}$.

   By the induction hypothesis we obtain the following.
   $\forall M_1 . M_1 \phi_1 \implies t_1,\sigma \handle{M_1 \simi} {t_1'},{\sigma'}\land M_1 \simt_1'\equiv{t_1'}\land M_1\sims' \equiv {\sigma'}$.

   Since $M$ satisfies $\phi_1$, we obtain from \refrule{H-FirstAnd} and the induction step above that
   $t_1\And t_2,\sigma\handle{M\First \simi}t_1'\And t_2,\sigma'$ with
   $M \simt_1'\And t_2\equiv {t_1'}\And t_2$ and $M\sims'\equiv {\sigma'}$.


   For all mappings $M$ such that $M\phi_2$, we need to demonstrate that
   $t_1\And t_2,\sigma\handle{M\Second \simi}t_1\And t_2',\sigma'$ with
   $M t_1\And \simt_2'\equiv t_1\And t_2'$ and $M\sims'\equiv {\sigma'}$.

  By the induction hypothesis we obtain the following.
  $\forall M_1 . M_1 \phi_1 \implies t_2,\sims \handle{M_1 \simi} {t_2'},{\sigma'}\land M_1 \simt_2'\equiv{t_2'}\land M_1\sims' \equiv {\sigma'}$

  Since $M$ satisfies $\phi_2$, we obtain from \refrule{H-SecondAnd} and the induction step above that
  $t_1\And t_2,\sigma\handle{M\Second \simi}t_1\And t_2',\sigma'$ with
  $M t_1\And \simt_2'\equiv t_1\And t_2'$ and $M\sims'\equiv {\sigma'}$.
  }

  \case{\refrule{SH-Or}}
  {This case is proven in the same way as \refrule{SH-And}.
  }


\end{proof}


\subsection{Proof of soundness of symbolic interacting semantics}
\begin{proof}
  We prove Theorem 6.1 by induction on $\simt,\sims\siminteract \overline{\simt',
  \sims',\simi,\phi}$.
  There is only one rule that applies, namely
  \refrule{SI-Handle}.

  Provided that $M(\phi_1\land\phi_2)$, we need to demonstrate that
  $t,\sigma\interact{M\simi}t'',\sigma''$ with
  $M \simt'' \equiv {t''}$ and $M\sims''\equiv {\sigma''}$.


  Lemma 6.3 and Lemma 6.2 respectively give us that\\
$\forall M_1 . M_1 \phi_1 \implies t,\sigma \handle{M_1 \simi} {t'},{\sigma'}\land M_1 \simt'\equiv{t'}\land M_1\sims' \equiv {\sigma'}$ and
$\forall M_2 . M_2 \phi_2 \implies t',\sigma' {\normalise} {t''},{\sigma''}\land M_2 \simt''\equiv{t''}\land M_2\sims'' \equiv {\sigma''}$.

Since $M$ satisfies both $\phi_1$ and $\phi_2$,
we obtain exactly what we need to prove,
namely
$t,\sigma\interact{\simi}t'',\sigma''$
$M \simt'' \equiv {t''}$ and $M\sims''\equiv {\sigma''}$.

\end{proof}
